define get_fun_pos_alt by map.fold, but turns out to be useless,
because adding or removing an element to the env (which happens
during proofs by induction) might completely change the iteration
order

compiler/src/compiler/FlatToRiscvDef.v
@@ -307,7 +307,7 @@ Section FlatToRiscv1.
       (old_insts ++ new_insts, map.put posmap fname pos).
 
     Definition compile_funs: env -> list Instruction * fun_pos_env :=
-      map.fold add_compiled_function (nil, e).
+      map.fold add_compiled_function (nil, map.empty).
   End WithEnv.
 
   (* compiles all functions just to obtain their code size *)
